ETCS_Base_FOL.thy
@@ -1,0 +1,353 @@
+theory ETCS_Base_FOL
+  imports FOL
+begin
+
+typedecl cset
+typedecl cfunc
+
+axiomatization
+  d0   :: "cfunc => cset" and
+  d1   :: "cfunc => cset" and
+  comp :: "cfunc => cfunc => cfunc"  (infixr "o" 55) and
+  id   :: "cset => cfunc"
+where
+  d0_comp:
+    "d1 (f) = d0 g --> d0 (g o f) = d0 f" and
+  d1_comp:
+    "d1 f = d0 g --> d1 (g o f) = d1 g" and
+  comp_associative:
+    "d1 f = d0 g --> d1 g = d0 h --> h o (g o f) = (h o g) o f" and
+  id_d0:
+    "d0 (id X) = X" and
+  id_d1:
+    "d1 (id X) = X" and
+  id_right_unit:
+    "f o id (d0 f) = f" and
+  id_left_unit:
+    "id (d1 f) o f = f"
+
+definition cfunc_type :: "[cfunc, cset, cset] \<Rightarrow> o" ("_ : _ \<rightarrow> _" [50, 50, 50] 50) where
+  "f : X \<rightarrow> Y \<equiv> (d0(f) = X \<and> d1(f) = Y)"
+
+lemma comp_type:
+  "f : X \<rightarrow> Y \<Longrightarrow> g : Y \<rightarrow> Z \<Longrightarrow> g \<circ> f : X \<rightarrow> Z"
+  by (simp add: cfunc_type_def d0_comp d1_comp)
+
+lemma comp_associative2:
+  "f : X \<rightarrow> Y \<Longrightarrow> g : Y \<rightarrow> Z \<Longrightarrow> h : Z \<rightarrow> W \<Longrightarrow> h \<circ> (g \<circ> f) = (h \<circ> g) \<circ> f"
+  by (simp add: cfunc_type_def comp_associative)
+
+lemma id_type:
+  "id(X) : X \<rightarrow> X"
+  by (simp add: cfunc_type_def id_d0 id_d1)
+
+lemma id_right_unit2:
+  "f : X \<rightarrow> Y \<Longrightarrow> f \<circ> id(X) = f"
+  by (simp add: cfunc_type_def id_right_unit)
+
+lemma id_left_unit2:
+  "f : X \<rightarrow> Y \<Longrightarrow> id(Y) \<circ> f = f"
+  by (simp add: cfunc_type_def id_left_unit)
+
+subsection \<open>Basic category-theoretic predicates\<close>
+
+definition triangle_commutes ::
+  "[cset, cset, cset, cfunc, cfunc, cfunc] \<Rightarrow> o"
+where
+  "triangle_commutes(A, B, C, ab, bc, ac) \<equiv>
+     (ab : A \<rightarrow> B \<and> bc : B \<rightarrow> C \<and> ac : A \<rightarrow> C \<and> bc \<circ> ab = ac)"
+
+definition square_commutes ::
+  "[cset, cset, cset, cset, cfunc, cfunc, cfunc, cfunc] \<Rightarrow> o"
+where
+  "square_commutes(A, B, C, D, ab, bd, ac, cd) \<equiv>
+     (ab : A \<rightarrow> B \<and> bd : B \<rightarrow> D \<and> ac : A \<rightarrow> C \<and> cd : C \<rightarrow> D \<and> bd \<circ> ab = cd \<circ> ac)"
+
+definition is_pullback ::
+  "[cset, cset, cset, cset, cfunc, cfunc, cfunc, cfunc] \<Rightarrow> o"
+where
+  "is_pullback(A, B, C, D, ab, bd, ac, cd) \<equiv>
+     (square_commutes(A, B, C, D, ab, bd, ac, cd) \<and>
+      (\<forall> Z k h.
+         (k : Z \<rightarrow> B \<and> h : Z \<rightarrow> C \<and> bd \<circ> k = cd \<circ> h) \<longrightarrow>
+         (\<exists>! j. j : Z \<rightarrow> A \<and> ab \<circ> j = k \<and> ac \<circ> j = h)))"
+
+definition monomorphism :: "cfunc \<Rightarrow> o" where
+  "monomorphism(f) \<equiv>
+     (\<forall> g h.
+        (d1(g) = d0(f) \<and> d1(h) = d0(f)) \<longrightarrow>
+        (f \<circ> g = f \<circ> h \<longrightarrow> g = h))"
+
+lemma monomorphism_def2:
+  "monomorphism(f) \<longleftrightarrow>
+     (\<forall> g h A X Y.
+        g : A \<rightarrow> X \<and> h : A \<rightarrow> X \<and> f : X \<rightarrow> Y \<longrightarrow>
+        (f \<circ> g = f \<circ> h \<longrightarrow> g = h))"
+  unfolding monomorphism_def cfunc_type_def
+  by blast
+
+lemma monomorphism_def3:
+  assumes "f : X \<rightarrow> Y"
+  shows "monomorphism(f) \<longleftrightarrow>
+           (\<forall> g h A.
+              g : A \<rightarrow> X \<and> h : A \<rightarrow> X \<longrightarrow>
+              (f \<circ> g = f \<circ> h \<longrightarrow> g = h))"
+  using assms
+  unfolding monomorphism_def2 cfunc_type_def
+  by blast
+
+definition epimorphism :: "cfunc \<Rightarrow> o" where
+  "epimorphism(f) \<equiv>
+     (\<forall> g h.
+        (d0(g) = d1(f) \<and> d0(h) = d1(f)) \<longrightarrow>
+        (g \<circ> f = h \<circ> f \<longrightarrow> g = h))"
+
+lemma epimorphism_def2:
+  "epimorphism(f) \<longleftrightarrow>
+     (\<forall> g h A X Y.
+        f : X \<rightarrow> Y \<and> g : Y \<rightarrow> A \<and> h : Y \<rightarrow> A \<longrightarrow>
+        (g \<circ> f = h \<circ> f \<longrightarrow> g = h))"
+  unfolding epimorphism_def cfunc_type_def
+  by blast
+
+lemma epimorphism_def3:
+  assumes "f : X \<rightarrow> Y"
+  shows "epimorphism(f) \<longleftrightarrow>
+           (\<forall> g h A.
+              g : Y \<rightarrow> A \<and> h : Y \<rightarrow> A \<longrightarrow>
+              (g \<circ> f = h \<circ> f \<longrightarrow> g = h))"
+  using assms
+  unfolding epimorphism_def2 cfunc_type_def
+  by blast
+
+subsection \<open>Isomorphisms (relational inverse, not THE)\<close>
+
+definition inverse_of :: "[cfunc, cfunc] \<Rightarrow> o" where
+  "inverse_of(g, f) \<equiv>
+     (g : d1(f) \<rightarrow> d0(f) \<and>
+      g \<circ> f = id(d0(f)) \<and>
+      f \<circ> g = id(d1(f)))"
+
+definition isomorphism :: "cfunc \<Rightarrow> o" where
+  "isomorphism(f) \<equiv> (\<exists> g. inverse_of(g, f))"
+
+lemma inverse_of_type:
+  "inverse_of(g, f) \<Longrightarrow> g : d1(f) \<rightarrow> d0(f)"
+  by (simp add: inverse_of_def)
+
+lemma inverse_of_sym:
+  assumes "inverse_of(g, f)"
+  shows "inverse_of(f, g)"
+proof -
+  from assms have g_ty: "g : d1(f) \<rightarrow> d0(f)"
+    and gf: "g \<circ> f = id(d0(f))"
+    and fg: "f \<circ> g = id(d1(f))"
+    unfolding inverse_of_def by blast+
+  have f_ty: "f : d0(f) \<rightarrow> d1(f)"
+    by (simp add: cfunc_type_def)
+  from g_ty have "d0(g) = d1(f)" and "d1(g) = d0(f)"
+    by (simp_all add: cfunc_type_def)
+  with f_ty gf fg show ?thesis
+    unfolding inverse_of_def cfunc_type_def
+    by simp
+qed
+
+lemma inverse_of_unique:
+  assumes gf: "inverse_of(g, f)"
+    and hf: "inverse_of(h, f)"
+  shows "g = h"
+proof -
+  from gf have g_ty: "g : d1(f) \<rightarrow> d0(f)"
+    and gf1: "g \<circ> f = id(d0(f))"
+    and gf2: "f \<circ> g = id(d1(f))"
+    unfolding inverse_of_def by blast+
+  from hf have h_ty: "h : d1(f) \<rightarrow> d0(f)"
+    and hf1: "h \<circ> f = id(d0(f))"
+    and hf2: "f \<circ> h = id(d1(f))"
+    unfolding inverse_of_def by blast+
+  have f_ty: "f : d0(f) \<rightarrow> d1(f)"
+    by (simp add: cfunc_type_def)
+
+  have "g = id(d0(f)) \<circ> g"
+    using g_ty by (simp add: id_left_unit2)
+  also have "... = (h \<circ> f) \<circ> g"
+    by (simp add: hf1)
+  also have "... = h \<circ> (f \<circ> g)"
+    by (rule sym, rule comp_associative2[OF g_ty f_ty h_ty])
+  also have "... = h \<circ> id(d1(f))"
+    by (simp add: gf2)
+  also have "... = h"
+    using h_ty by (simp add: id_right_unit2)
+  finally show "g = h" .
+qed
+
+lemma isomorphism_def2:
+  "isomorphism(f) \<longleftrightarrow>
+     (\<exists> g X Y.
+        f : X \<rightarrow> Y \<and> g : Y \<rightarrow> X \<and>
+        g \<circ> f = id(X) \<and> f \<circ> g = id(Y))"
+  unfolding isomorphism_def inverse_of_def
+  by (blast simp add: cfunc_type_def)
+
+lemma isomorphism_def3:
+  assumes "f : X \<rightarrow> Y"
+  shows "isomorphism(f) \<longleftrightarrow>
+           (\<exists> g.
+              g : Y \<rightarrow> X \<and>
+              g \<circ> f = id(X) \<and>
+              f \<circ> g = id(Y))"
+  using assms
+  unfolding isomorphism_def2 cfunc_type_def
+  by blast
+
+definition is_isomorphic :: "[cset, cset] \<Rightarrow> o" (infix "\<cong>" 50) where
+  "X \<cong> Y \<equiv> (\<exists> f. f : X \<rightarrow> Y \<and> isomorphism(f))"
+
+lemma id_isomorphism:
+  "isomorphism(id(X))"
+proof -
+  have "inverse_of(id(X), id(X))"
+    unfolding inverse_of_def
+    by (simp add: id_type id_left_unit2 id_right_unit2)
+  thus ?thesis
+    unfolding isomorphism_def
+    by blast
+qed
+
+lemma isomorphic_is_reflexive:
+  "X \<cong> X"
+  unfolding is_isomorphic_def
+  by (blast intro: id_type id_isomorphism)
+
+lemma isomorphic_is_symmetric:
+  "X \<cong> Y \<Longrightarrow> Y \<cong> X"
+  unfolding is_isomorphic_def isomorphism_def
+  by (blast intro: inverse_of_sym)
+
+subsection \<open>Representative transported lemmas\<close>
+
+lemma comp_monic_imp_monic:
+  assumes "d1(f) = d0(g)"
+  shows "monomorphism(g \<circ> f) \<Longrightarrow> monomorphism(f)"
+  unfolding monomorphism_def
+proof clarify
+  fix s t
+  assume gf_monic:
+    "\<forall> s t.
+       (d1(s) = d0(g \<circ> f) \<and> d1(t) = d0(g \<circ> f)) \<longrightarrow>
+       ((g \<circ> f) \<circ> s = (g \<circ> f) \<circ> t \<longrightarrow> s = t)"
+  assume s_ty: "d1(s) = d0(f)"
+  assume t_ty: "d1(t) = d0(f)"
+  assume fst_eq: "f \<circ> s = f \<circ> t"
+
+  have "(g \<circ> f) \<circ> s = (g \<circ> f) \<circ> t"
+    using fst_eq assms s_ty t_ty
+    by (blast intro: comp_associative)
+  thus "s = t"
+    using gf_monic s_ty t_ty assms d0_comp
+    by simp
+qed
+
+lemma comp_epi_imp_epi:
+  assumes "d1(f) = d0(g)"
+  shows "epimorphism(g \<circ> f) \<Longrightarrow> epimorphism(g)"
+  unfolding epimorphism_def
+proof clarify
+  fix s t
+  assume gf_epi:
+    "\<forall> s t.
+       (d0(s) = d1(g \<circ> f) \<and> d0(t) = d1(g \<circ> f)) \<longrightarrow>
+       (s \<circ> (g \<circ> f) = t \<circ> (g \<circ> f) \<longrightarrow> s = t)"
+  assume s_ty: "d0(s) = d1(g)"
+  assume t_ty: "d0(t) = d1(g)"
+  assume sg_tg: "s \<circ> g = t \<circ> g"
+
+  have "s \<circ> (g \<circ> f) = t \<circ> (g \<circ> f)"
+    using sg_tg assms s_ty t_ty
+    by (simp add: comp_associative)
+  thus "s = t"
+    using gf_epi s_ty t_ty assms d1_comp
+    by simp
+qed
+
+lemma iso_imp_epi_and_monic:
+  "isomorphism(f) \<Longrightarrow> epimorphism(f) \<and> monomorphism(f)"
+  unfolding isomorphism_def
+proof
+  assume "\<exists> g. inverse_of(g, f)"
+  then obtain g where inv: "inverse_of(g, f)"
+    by blast
+
+  from inv have g_ty: "g : d1(f) \<rightarrow> d0(f)"
+    and gf_id: "g \<circ> f = id(d0(f))"
+    and fg_id: "f \<circ> g = id(d1(f))"
+    unfolding inverse_of_def by blast+
+
+  have f_ty: "f : d0(f) \<rightarrow> d1(f)"
+    by (simp add: cfunc_type_def)
+
+  show "epimorphism(f) \<and> monomorphism(f)"
+  proof (rule conjI)
+    show "epimorphism(f)"
+      unfolding epimorphism_def
+    proof clarify
+      fix s t
+      assume s_ty: "d0(s) = d1(f)"
+      assume t_ty: "d0(t) = d1(f)"
+      assume sf_tf: "s \<circ> f = t \<circ> f"
+
+      have s_type: "s : d1(f) \<rightarrow> d1(s)"
+        using s_ty by (simp add: cfunc_type_def)
+      have t_type: "t : d1(f) \<rightarrow> d1(t)"
+        using t_ty by (simp add: cfunc_type_def)
+
+      have "s = s \<circ> id(d1(f))"
+        using s_type by (simp add: id_right_unit2)
+      also have "... = s \<circ> (f \<circ> g)"
+        by (simp add: fg_id)
+      also have "... = (s \<circ> f) \<circ> g"
+        by (rule comp_associative2[OF g_ty f_ty s_type])
+      also have "... = (t \<circ> f) \<circ> g"
+        by (simp add: sf_tf)
+      also have "... = t \<circ> (f \<circ> g)"
+        by (rule sym, rule comp_associative2[OF g_ty f_ty t_type])
+      also have "... = t \<circ> id(d1(f))"
+        by (simp add: fg_id)
+      also have "... = t"
+        using t_type by (simp add: id_right_unit2)
+      finally show "s = t" .
+    qed
+
+    show "monomorphism(f)"
+      unfolding monomorphism_def
+    proof clarify
+      fix h k
+      assume h_ty: "d1(h) = d0(f)"
+      assume k_ty: "d1(k) = d0(f)"
+      assume fh_fk: "f \<circ> h = f \<circ> k"
+
+      have h_type: "h : d0(h) \<rightarrow> d0(f)"
+        using h_ty by (simp add: cfunc_type_def)
+      have k_type: "k : d0(k) \<rightarrow> d0(f)"
+        using k_ty by (simp add: cfunc_type_def)
+
+      have "h = id(d0(f)) \<circ> h"
+        using h_type by (simp add: id_left_unit2)
+      also have "... = (g \<circ> f) \<circ> h"
+        by (simp add: gf_id)
+      also have "... = g \<circ> (f \<circ> h)"
+        by (rule comp_associative2[OF h_type f_ty g_ty])
+      also have "... = g \<circ> (f \<circ> k)"
+        by (simp add: fh_fk)
+      also have "... = (g \<circ> f) \<circ> k"
+        by (rule sym, rule comp_associative2[OF k_type f_ty g_ty])
+      also have "... = id(d0(f)) \<circ> k"
+        by (simp add: gf_id)
+      also have "... = k"
+        using k_type by (simp add: id_left_unit2)
+      finally show "h = k" .
+    qed
+  qed
+qed
+
+end
